prove the serializer examples

src/lowparse/LowParse.Spec.Fold.fst
@@ -49,6 +49,8 @@ let get (#state_t: Type) () : Tot (stt state_t (Ghost.erased state_t) (fun _ -> 
 
 let skip (#state_t: Type) () : Tot (stt state_t unit (fun _ -> True) (fun _ _ _ -> True)) = ret ()
 
+let state_assert (#state_t: Type) (p: state_t -> prop) : Tot (stt state_t unit p (fun s _ s' -> s == s' /\ p s)) = fun s -> ((), s)
+
 let bind (#state_t: Type) (#ret1_t #ret2_t: Type)
   (#pre1: state_t -> prop)
   (#post1: state_t -> ret1_t -> state_t -> prop)
@@ -76,15 +78,17 @@ let fold_t (state_t: Type) (t: Type) (ret_t: Type) (pre: state_t -> prop) (post:
 let fold_pair_post
   (#state_t: Type)
   #t1 #ret1
+  (pre1: state_t -> prop)
   (post1: t1 -> state_t -> ret1 -> state_t -> prop)
   #t2 #ret2
+  (pre2: ret1 -> state_t -> prop)
   (post2: (x: ret1) -> t2 -> state_t -> ret2 -> state_t -> prop)
   (v: (t1 & t2))
   (s0: state_t)
   (r2: ret2)
   (s2: state_t)
 : Tot prop
-= exists s1 r1 . post1 (fst v) s0 r1 s1 /\ post2 r1 (snd v) s1 r2 s2
+= pre1 s0 /\ (exists s1 r1 . post1 (fst v) s0 r1 s1 /\ pre2 r1 s1 /\ post2 r1 (snd v) s1 r2 s2)
 
 let fold_pair
   (#state_t: Type)
@@ -92,7 +96,7 @@ let fold_pair
   (f1: fold_t state_t t1 ret1 pre1 post1)
   #t2 #ret2 (#pre2: ret1 -> _) (#post2: ret1 -> _)
   (f2: (x: ret1) -> fold_t state_t t2 ret2 (pre2 x) (post2 x))
-: Pure (fold_t state_t (t1 & t2) ret2 pre1 (fold_pair_post post1 post2))
+: Pure (fold_t state_t (t1 & t2) ret2 pre1 (fold_pair_post pre1 post1 pre2 post2))
     (requires (
       (forall s v1 r1 s' . post1 v1 s r1 s' ==> pre2 r1 s')
     ))
@@ -136,15 +140,17 @@ let fold_choice
 let bind_fold_post
   (#state_t: Type)
   #t #ret1
+  (pre1: state_t -> prop)
   (post1: t -> state_t -> ret1 -> state_t -> prop)
   #ret2
+  (pre2: ret1 -> state_t -> prop)
   (post2: (x: ret1) -> t -> state_t -> ret2 -> state_t -> prop)
   (v: t)
   (s0: state_t)
   (r2: ret2)
   (s2: state_t)
 : Tot prop
-= exists s1 r1 . post1 v s0 r1 s1 /\ post2 r1 v s1 r2 s2
+= pre1 s0 /\ (exists s1 r1 . post1 v s0 r1 s1 /\ pre2 r1 s1 /\ post2 r1 v s1 r2 s2)
 
 let bind_fold
   (#state_t: Type)
@@ -157,7 +163,7 @@ let bind_fold
   (#post2: _)
   (f: fold_t state_t t ret1 pre1 post1)
   (g: (x: ret1) -> fold_t state_t t ret2 (pre2 x) (post2 x))
-: Pure (fold_t state_t t ret2 pre1 (bind_fold_post post1 post2))
+: Pure (fold_t state_t t ret2 pre1 (bind_fold_post pre1 post1 pre2 post2))
     (requires (forall s v r s' . post1 s v r s' ==> pre2 r s'))
     (ensures (fun _ -> True))
 = fun v s0 ->
@@ -207,7 +213,7 @@ type prog
       (g: ((x: ret1) -> prog state_t action_impl_t t ret2 (pre2 x) (post2 x)) {
         forall s v r s' . post1 s v r s' ==> pre2 r s'
       }) ->
-      prog state_t action_impl_t t ret2 pre1 (bind_fold_post post1 post2)
+      prog state_t action_impl_t t ret2 pre1 (bind_fold_post pre1 post1 pre2 post2)
   | PU8:
       (#ret_t: _) -> (#pre: _) -> (#post: _) ->
       ((x: U8.t) -> action state_t action_impl_t ret_t pre (post x)) ->
@@ -225,7 +231,7 @@ type prog
       (f2: ((x: ret1) -> prog state_t action_impl_t t2 ret2 (pre2 x) (post2 x)) {
         forall s v1 r1 s' . post1 v1 s r1 s' ==> pre2 r1 s'
       }) ->
-      prog state_t action_impl_t (TPair t1 t2) ret2 pre1 (fold_pair_post post1 post2)
+      prog state_t action_impl_t (TPair t1 t2) ret2 pre1 (fold_pair_post pre1 post1 pre2 post2)
   | PList:
       (#t: typ) ->
       (#inv: _) ->
@@ -260,62 +266,148 @@ let rec sem
 
 noeq
 type base_context_t
+  (erase_values: bool)
   : typ -> typ -> Type
-= | CPairL: (l: typ) -> (r: typ) -> base_context_t (TPair l r) l
-  | CPairR: (l: typ) -> (vl: type_of_typ l) -> (r: typ) -> base_context_t (TPair l r) r
-  | CListCons: (t: typ) -> (l: list (type_of_typ t)) -> base_context_t (TList t) t
-  | CChoicePayload: (f: (bool -> typ)) -> (tag: bool) -> base_context_t (TChoice f) (f tag)
+= | CPairL: (l: typ) -> (r: typ) -> base_context_t erase_values (TPair l r) l
+  | CPairR: (l: typ) -> (vl: (if erase_values then unit else type_of_typ l)) -> (r: typ) -> base_context_t erase_values (TPair l r) r
+  | CListCons: (t: typ) -> (l: (if erase_values then unit else list (type_of_typ t))) -> base_context_t erase_values (TList t) t
+  | CChoicePayload: (f: (bool -> typ)) -> (tag: bool) -> base_context_t erase_values (TChoice f) (f tag)
+
+let base_context_erase_values
+  (#erase_values: bool)
+  (#t1: _)
+  (#t2: _)
+  (x: base_context_t erase_values t1 t2)
+: Tot (base_context_t true t1 t2)
+= match x with
+  | CPairL l r -> CPairL l r
+  | CPairR l _ r -> CPairR l () r
+  | CListCons t _ -> CListCons t ()
+  | CChoicePayload f tag -> CChoicePayload f tag
 
 noeq
 type context_t
+  (erase_values: bool)
   : typ -> typ -> Type
-= | CNil: (#t: typ) -> context_t t t
-  | CSnoc: (#t1: typ) -> (#t2: typ) -> (#t3: typ) -> context_t t1 t2 -> base_context_t t2 t3 -> context_t t1 t3
+= | CNil: (#t: typ) -> context_t erase_values t t
+  | CSnoc: (#t1: typ) -> (#t2: typ) -> (#t3: typ) -> context_t erase_values t1 t2 -> base_context_t erase_values t2 t3 -> context_t erase_values t1 t3
+
+let rec context_erase_values
+  (#erase_values: bool)
+  (#t1 #t2: _)
+  (x: context_t erase_values t1 t2)
+: Tot (context_t true t1 t2)
+  (decreases x)
+= match x with
+  | CNil -> CNil
+  | CSnoc c b -> CSnoc (context_erase_values c) (base_context_erase_values b)
 
 let rec concat_context
+  (#erase_values: bool)
   (#t1 #t2 #t4: typ)
-  (c12: context_t t1 t2)
-  (c24: context_t t2 t4)
-: Tot (context_t t1 t4)
+  (c12: context_t erase_values t1 t2)
+  (c24: context_t erase_values t2 t4)
+: Tot (context_t erase_values t1 t4)
   (decreases c24)
 = match c24 with
   | CNil -> c12
   | CSnoc c23 b34 -> CSnoc (concat_context c12 c23) b34
 
+let rec erase_values_concat_context
+  (#erase_values: bool)
+  (#t1 #t2 #t4: typ)
+  (c12: context_t erase_values t1 t2)
+  (c24: context_t erase_values t2 t4)
+: Lemma
+  (requires True)
+  (ensures (context_erase_values (c12 `concat_context` c24) == context_erase_values c12 `concat_context` context_erase_values c24))
+  (decreases c24)
+= match c24 with
+  | CNil -> ()
+  | CSnoc c23 b34 -> erase_values_concat_context c12 c23
+
 noeq
 type base_hole_t
+  (erase_values: bool)
   : typ -> Type
-= | HU8: base_hole_t TU8
-  | HList: (t: typ) -> (l: list (type_of_typ t)) -> base_hole_t (TList t)
-  | HChoiceTag: (f: (bool -> typ)) -> base_hole_t (TChoice f)
+= | HU8: base_hole_t erase_values TU8
+  | HList: (t: typ) -> (l: (if erase_values then unit else list (type_of_typ t))) -> base_hole_t erase_values (TList t)
+  | HChoiceTag: (f: (bool -> typ)) -> base_hole_t erase_values (TChoice f)
+
+let base_hole_erase_values
+  (#erase_values: bool)
+  (#t: typ)
+  (x: base_hole_t erase_values t)
+: Tot (base_hole_t true t)
+= match x with
+  | HU8 -> HU8
+  | HList t _ -> HList t ()
+  | HChoiceTag f -> HChoiceTag f
 
 noeq
 type hole_t
+  (erase_values: bool)
 = {
   root: typ;
   leaf: typ;
-  context: context_t root leaf;
-  hole: base_hole_t leaf;
+  context: context_t erase_values root leaf;
+  hole: base_hole_t erase_values leaf;
+}
+
+let hole_erase_values
+  (#erase_values: bool)
+  (x: hole_t erase_values)
+: Tot (hole_t true)
+= {
+  root = x.root;
+  leaf = x.leaf;
+  context = context_erase_values x.context;
+  hole = base_hole_erase_values x.hole;
 }
 
 let rec init_hole
+  (erase_values: bool)
   (t: typ)
-: Pure hole_t
+: Pure (hole_t erase_values)
   (requires True)
   (ensures (fun res -> res.root == t))
 = match t with
   | TU8 -> { root = TU8; leaf = TU8; context = CNil; hole = HU8 }
-  | TList t -> { root = TList t; leaf = TList t; context = CNil; hole = HList t [] }
+  | TList t -> { root = TList t; leaf = TList t; context = CNil; hole = HList t (if erase_values then () else ([] <: list (type_of_typ t))) }
   | TChoice f -> { root = TChoice f; leaf = TChoice f; context = CNil; hole = HChoiceTag f }
   | TPair l r ->
-    let h = init_hole l in
+    let h = init_hole erase_values l in
     { root = TPair l r; leaf = h.leaf; context = concat_context (CSnoc CNil (CPairL l r)) h.context; hole = h.hole }
+
+let rec erase_values_init_hole
+  (erase_values: bool)
+  (t: typ)
+: Lemma
+  (hole_erase_values (init_hole erase_values t) == init_hole true t)
+= match t with
+  | TU8 -> ()
+  | TList t -> ()
+  | TChoice f -> ()
+  | TPair l r ->
+    erase_values_init_hole erase_values l;
+    let h = init_hole erase_values l in
+    erase_values_concat_context (CSnoc CNil (CPairL l r)) h.context
 
 noeq
 type hole_or_value_t
+  (erase_values: bool)
   (t: typ)
-= | Value: type_of_typ t -> hole_or_value_t t
-  | Hole: (h: hole_t { h.root == t }) -> hole_or_value_t t
+= | Value: (if erase_values then unit else type_of_typ t) -> hole_or_value_t erase_values t
+  | Hole: (h: hole_t erase_values { h.root == t }) -> hole_or_value_t erase_values t
+
+let hole_or_value_erase_values
+  (#erase_values: _)
+  (#t: typ)
+  (h: hole_or_value_t erase_values t)
+: Tot (hole_or_value_t true t)
+= match h with
+  | Value _ -> Value ()
+  | Hole h -> Hole (hole_erase_values h)
 
 let mk_choice_value
   (tag: bool)
@@ -325,58 +417,93 @@ let mk_choice_value
 = (| tag, v |)
 
 let rec fill_context
+  (#erase_values: bool)
   (#root: typ)
   (#leaf: typ)
-  (c: context_t root leaf)
-  (v: type_of_typ leaf)
-: Tot (hole_or_value_t root)
+  (c: context_t erase_values root leaf)
+  (v: (if erase_values then unit else type_of_typ leaf))
+: Tot (hole_or_value_t erase_values root)
   (decreases c)
 = match c with
   | CNil ->
     Value v
   | CSnoc c' (CPairL l r) ->
-    let h = init_hole r in
+    let h = init_hole erase_values r in
     Hole ({ root = root; leaf = h.leaf; context = concat_context (CSnoc c' (CPairR l v r)) h.context; hole = h.hole })
   | CSnoc c' (CPairR l vl r) ->
-    fill_context c' (vl, v)
+    fill_context c' (if erase_values then () else (vl, v))
   | CSnoc c' (CListCons t l) ->
-    Hole ({ root = root; leaf = _; context = c'; hole = HList t (l `List.Tot.append` [v] )})
+    Hole ({ root = root; leaf = _; context = c'; hole = HList t (if erase_values then () else l `List.Tot.append` [v] )})
   | CSnoc c' (CChoicePayload f tag) ->
-    fill_context c' (mk_choice_value tag f v)
+    fill_context c' (if erase_values then () else mk_choice_value tag f v)
+
+let rec erase_values_fill_context
+  (#erase_values: bool)
+  (#root: typ)
+  (#leaf: typ)
+  (c: context_t erase_values root leaf)
+  (v: (if erase_values then unit else type_of_typ leaf))
+: Lemma
+  (requires True)
+  (ensures (hole_or_value_erase_values (fill_context c v) == fill_context (context_erase_values c) ()))
+  (decreases c)
+= match c with
+  | CNil -> ()
+  | CSnoc c' (CPairL l r) ->
+    erase_values_init_hole erase_values r;
+    let h = init_hole erase_values r in
+    erase_values_concat_context (CSnoc c' (CPairR l v r)) h.context
+  | CSnoc c' (CPairR l vl r) ->
+    erase_values_fill_context c' (if erase_values then () else (vl, v))
+  | CSnoc c' (CListCons t l) -> ()
+  | CSnoc c' (CChoicePayload f tag) ->
+    erase_values_fill_context c' (if erase_values then () else mk_choice_value tag f v)
 
 let transition'_u8
-  (v: U8.t)
-  (h: hole_t { h.leaf == TU8 })
-: Tot (hole_or_value_t h.root)
+  (#erase_values: bool)
+  (h: hole_t erase_values { h.leaf == TU8 })
+  (v: (if erase_values then unit else U8.t))
+: Tot (hole_or_value_t erase_values h.root)
 = fill_context h.context v
 
 let transition_u8
   (t: typ)
   (v: U8.t)
-: Tot (stt (hole_or_value_t t) unit (fun s -> Hole? s /\ (Hole?.h s).leaf == TU8) (fun _ _ _ -> True))
+: Tot (stt (hole_or_value_t false t) unit (fun s -> Hole? s /\ (Hole?.h s).leaf == TU8) (fun s _ s' ->
+      Hole? s /\ (Hole?.h s).leaf == TU8 /\
+      hole_or_value_erase_values s' == transition'_u8 (Hole?.h (hole_or_value_erase_values s)) ()
+  ))
 = fun s ->
   let Hole h = s in
-  ((), transition'_u8 v h)
+  erase_values_fill_context h.context v;
+  ((), transition'_u8 h v)
 
 let transition'_list_nil
-  (h: hole_t { TList? h.leaf })
-: Tot (hole_or_value_t h.root)
+  (#erase_values: bool)
+  (h: hole_t erase_values { TList? h.leaf })
+: Tot (hole_or_value_t erase_values h.root)
 = let TList t = h.leaf in
-  fill_context h.context ([] <: list (type_of_typ t))
+  fill_context h.context (if erase_values then () else ([] <: list (type_of_typ t)))
 
 let transition_list_nil
   (t: typ)
-: Tot (stt (hole_or_value_t t) unit (fun s -> Hole? s /\ TList? (Hole?.h s).leaf) (fun _ _ _ -> True))
+: Tot (stt (hole_or_value_t false t) unit (fun s -> Hole? s /\ TList? (Hole?.h s).leaf) (fun s _ s' ->
+    Hole? s /\ TList? (Hole?.h s).leaf /\
+    hole_or_value_erase_values s' == transition'_list_nil (Hole?.h (hole_or_value_erase_values s))
+  ))
 = fun s ->
   let Hole h = s in
+  let TList t' = h.leaf in
+  erase_values_fill_context h.context ([] <: list (type_of_typ t'));
   ((), transition'_list_nil h)
 
 let transition'_list_cons
-  (h: hole_t { TList? h.leaf })
-: Tot (hole_or_value_t h.root)
+  (#erase_values: bool)
+  (h: hole_t erase_values { TList? h.leaf })
+: Tot (hole_or_value_t erase_values h.root)
 = let TList t = h.leaf in
   let HList _ l = h.hole in
-  let h' = init_hole t in
+  let h' = init_hole erase_values t in
   Hole ({
     root = h.root;
     leaf = h'.leaf;
@@ -386,17 +513,26 @@ let transition'_list_cons
 
 let transition_list_cons
   (t: typ)
-: Tot (stt (hole_or_value_t t) unit (fun s -> Hole? s /\ TList? (Hole?.h s).leaf) (fun _ _ _ -> True))
+: Tot (stt (hole_or_value_t false t) unit (fun s -> Hole? s /\ TList? (Hole?.h s).leaf) (fun s _ s' ->
+    Hole? s /\ TList? (Hole?.h s).leaf /\
+    hole_or_value_erase_values s' == transition'_list_cons (Hole?.h (hole_or_value_erase_values s))
+  ))
 = fun s ->
   let Hole h = s in
+  let TList t' = h.leaf in
+  let HList _ l = h.hole in
+  erase_values_init_hole false t';
+  let h' = init_hole false t' in
+  erase_values_concat_context (CSnoc h.context (CListCons t' l)) h'.context;
   ((), transition'_list_cons h)
 
 let transition'_choice_tag
-  (h: hole_t { TChoice? h.leaf })
+  (#erase_values: bool)
+  (h: hole_t erase_values { TChoice? h.leaf })
   (tag: bool)
-: Tot (hole_or_value_t h.root)
+: Tot (hole_or_value_t erase_values h.root)
 = let TChoice f = h.leaf in
-  let h' = init_hole (f tag) in
+  let h' = init_hole erase_values (f tag) in
   Hole ({
     root = h.root;
     leaf = h'.leaf;
@@ -407,9 +543,16 @@ let transition'_choice_tag
 let transition_choice_tag
   (t: typ)
   (tag: bool)
-: Tot (stt (hole_or_value_t t) unit (fun s -> Hole? s /\ TChoice? (Hole?.h s).leaf) (fun _ _ _ -> True))
+: Tot (stt (hole_or_value_t false t) unit (fun s -> Hole? s /\ TChoice? (Hole?.h s).leaf) (fun s _ s' ->
+    Hole? s /\ TChoice? (Hole?.h s).leaf /\
+    hole_or_value_erase_values s' == transition'_choice_tag (Hole?.h (hole_or_value_erase_values s)) tag
+  ))
 = fun s ->
   let Hole h = s in
+  let TChoice f = h.leaf in
+  erase_values_init_hole false (f tag);
+  let h' = init_hole false (f tag) in
+  erase_values_concat_context (CSnoc h.context (CChoicePayload f tag)) h'.context;
   ((), transition'_choice_tag h tag)
 
 let mk_unit_action
@@ -424,20 +567,18 @@ let mk_unit_action
   action_impl = ();
 }
 
-#push-options "--admit_smt_queries true"
-
-let _ : prog (hole_or_value_t (TPair TU8 TU8)) (fun _ _ _ _ -> unit) (TPair TU8 TU8) unit _ _ =
+let _ : prog (hole_or_value_t false (TPair TU8 TU8)) (fun _ _ _ _ -> unit) (TPair TU8 TU8) unit _ _ =
   PPair
-    (PU8 (fun x1 -> mk_unit_action (transition_u8 _ x1)))
+    (PBind
+      (PRet (mk_unit_action (state_assert (fun s -> s == Hole (init_hole false (TPair TU8 TU8))))))
+      (fun _ -> PU8 (fun x1 -> mk_unit_action (transition_u8 _ x1))))
     (fun _ -> PU8 (fun x2 -> mk_unit_action (transition_u8 _ x2)))
 
-let _ : prog (hole_or_value_t (TPair TU8 TU8)) (fun _ _ _ _ -> unit) (TPair TU8 TU8) unit _ _ =
+let _ : prog (hole_or_value_t false (TPair TU8 TU8)) (fun _ _ _ _ -> unit) (TPair TU8 TU8) unit _ _ =
   PBind
     (PPair
-      (PRet (mk_unit_action (ret ())))
+      (PRet (mk_unit_action (state_assert (fun s -> s == Hole (init_hole false (TPair TU8 TU8))))))
       (fun _ -> PU8 (fun x2 -> mk_unit_action (transition_u8 _ x2))))
     (fun _ -> PPair
-      (PU8 (fun x1 -> mk_unit_action (transition_u8 _ x1)))
-      (fun _ -> PRet (mk_unit_action (ret ()))))
-
-#pop-options
+       (PU8 (fun x1 -> mk_unit_action (transition_u8 _ x1)))
+       (fun _ -> PRet (mk_unit_action (ret ()))))
